src/Crypto/AESUtils.dfy
@@ -12,6 +12,10 @@ module {:extern "AESUtils"} AESUtils {
   const TAG_LEN := 16 as uint8;
   const IV_LEN := 12 as uint8;
 
+  const AES_GCM_128 := Params(AES128, 16, TAG_LEN, IV_LEN)
+  const AES_GCM_192 := Params(AES192, 24, TAG_LEN, IV_LEN)
+  const AES_GCM_256 := Params(AES256, 32, TAG_LEN, IV_LEN)
+
   function method KeyLengthOfCipher(m: Mode): uint8 {
     match m
     case AES256 => 32
