src/SDK/Keyring/AESWrappingSuite.dfy
@@ -1,0 +1,24 @@
+include "../../Crypto/AESUtils.dfy"
+include "../../StandardLibrary/StandardLibrary.dfy"
+include "../../Crypto/GenBytes.dfy"
+
+module AESKeyring.AESWrappingSuite {
+  import opened StandardLibrary
+  import opened UInt = StandardLibrary.UInt
+  import AES = AESUtils
+  import RNG
+
+  const VALID_ALGORITHMS := {AES.AES_GCM_128, AES.AES_GCM_192, AES.AES_GCM_256}
+
+  method GenIV(p: AES.Params) returns (s: seq<uint8>)
+    ensures |s| == p.ivLen as int
+  {
+    s := RNG.GenBytes(p.ivLen as uint16);
+  }
+
+  method GenKey(p: AES.Params) returns (s: seq<uint8>)
+    ensures |s| == p.keyLen as int
+  {
+    s := RNG.GenBytes(p.keyLen as uint16);
+  }
+}
